Restructure Unification (and minor upgrades)

matching-logic/src/Experimental/Unification.v
@@ -2,21 +2,14 @@ From MatchingLogic.Theories Require Export FOEquality_ProofSystem.
 Import MatchingLogic.Logic.Notations.
 Import MatchingLogic.Theories.Definedness_Syntax.Notations.
 
+From MatchingLogic Require Export Unification.Definitions.
+
 Set Default Proof Mode "Classic".
 
 Close Scope equations_scope. (* Because of [!] *)
 
 Section unification.
   Context {Σ : Signature} {syntax : Syntax}.
-
-  Section helpers.
-
-    Definition get_fresh_evar (φ : Pattern) : sig (.∉ free_evars φ).
-    Proof.
-      exists (fresh_evar φ); auto.
-    Defined.
-
-  End helpers.
 
   (** The naming of the following lemmas matches this article:
         Unification in Matching Logic - Extended Version
@@ -62,24 +55,6 @@ Section unification.
       mlExact "H1".
   Defined.
 
-  Definition substitute_list (σ : list (evar * Pattern)) (t : Pattern) : Pattern := fold_left (fun φ '(x, φ') => φ^[[evar: x ↦ φ']]) σ t.
-
-  Lemma wf_substitute_list : forall σ t, wf (map snd σ) -> well_formed t -> well_formed (substitute_list σ t).
-  Proof.
-    intros.
-    apply wf_fold_left with (t := snd); try assumption.
-    intros ? [] **; wf_auto2.
-  Qed.
-
-  Definition predicate_list (σ : list (evar * Pattern)) : Pattern := fold_right (fun '(x, φ') φ => patt_free_evar x =ml φ' and φ) patt_top σ.
-
-  Lemma wf_predicate_list : forall σ, wf (map snd σ) -> well_formed (predicate_list σ).
-  Proof.
-    intros.
-    apply wf_foldr with (t := snd);
-    only 3: intros ? [] **; wf_auto2.
-  Qed.
-  
   Lemma Lemma₁ : forall Γ φ t x, theory ⊆ Γ ->
     well_formed φ ->
     mu_free φ ->
@@ -87,23 +62,23 @@ Section unification.
     Γ ⊢ (patt_free_evar x) =ml t ---> φ^[[evar:x↦t]] =ml φ.
   Proof.
     intros * HΓ wfφ mfφ wft.
-    pose proof (get_fresh_evar φ) as [y Hy].
+    mlFreshEvar as y.
     pose proof (equality_elimination_basic Γ (patt_free_evar x) t {| pcEvar := y; pcPattern := φ^[[evar: x ↦ patt_free_evar y]] =ml φ |}).
     ospecialize* H; auto. wf_auto2.
     simpl. now erewrite mu_free_free_evar_subst, mfφ.
     cbn -["=ml"] in H. mlSimpl in H.
-    erewrite ! free_evar_subst_chain, free_evar_subst_id, ! (free_evar_subst_no_occurrence y) in H by auto.
+    erewrite ! free_evar_subst_chain, free_evar_subst_id, ! (free_evar_subst_no_occurrence y) in H by ltac2:(fm_solve()).
     mlIntro "H".
     mlApplyMeta H in "H".
     mlDestructAnd "H" as "H1" "H2".
     mlApply "H1". mlReflexivity.
   Defined.
 
-  Lemma Lemma₂ : forall Γ φ σ (i : ProofInfo),
+  Lemma Lemma₂ : forall Γ φ σ,
     theory ⊆ Γ -> mu_free φ -> well_formed φ ->
     forallb mu_free (map snd σ) -> wf (map snd σ) ->
     Γ ⊢i substitute_list σ φ and predicate_list σ <--->
-      φ and predicate_list σ using i.
+      φ and predicate_list σ using AnyReasoning.
   Proof.
     intros * HΓ mfφ wfφ mfσ wfσ.
     pose proof (wf_predicate_list σ wfσ) as WF1.
@@ -121,159 +96,15 @@ Section unification.
     mlApplyMeta (pf_iff_equiv_trans_obj) in "H2".
     mlApply "H2". mlClear "H2".
     epose proof (Lemma₁ _ φ _ _ _ _ _ _).
-    mlApplyMeta H in "H1". clear H. 2: admit.
+    mlApplyMeta H in "H1". clear H.
     epose proof (get_fresh_evar (φ^[[evar:e↦p]] <---> φ)) as [y Hy].
     epose proof (total_phi_impl_phi _ _ _ _ Hy _).
     mlApplyMeta H in "H1". clear H.
-    mlExact "H1". admit.
+    mlExact "H1".
     Unshelve. all: try solve [auto | wf_auto2].
+    1,3: exact AnyReasoning.
     simpl in mfσ. apply andb_true_iff in mfσ as [].
     apply mu_free_free_evar_subst; auto.
-  Admitted.
-
-  Definition is_unifier_of (σ : list (evar * Pattern)) t₁ t₂ := substitute_list σ t₁ =ml substitute_list σ t₂.
-
-  Lemma wf_is_unifier_of : forall σ t₁ t₂, wf (map snd σ) -> well_formed t₁ -> well_formed t₂ -> well_formed (is_unifier_of σ t₁ t₂).
-  Proof.
-    intros.
-    apply well_formed_equal; apply wf_substitute_list; assumption.
-  Qed.
-
-  Lemma predicate_list_predicate Γ σ : theory ⊆ Γ -> wf (map snd σ) -> Γ ⊢ is_predicate_pattern (predicate_list σ).
-  Proof with wf_auto2.
-    intros HΓ wfσ.
-    epose proof (foldr_ind_set (λ φ, well_formed φ -> Γ ⊢ is_predicate_pattern φ) (λ '(x, φ), well_formed (patt_free_evar x =ml φ) -> Γ ⊢ is_predicate_pattern (patt_free_evar x =ml φ)) (λ '(x, φ') (φ : Pattern), patt_free_evar x =ml φ' and φ) patt_top σ).
-    ospecialize* X. 1-4: clear X.
-    * intro. toMLGoal... mlLeft. mlReflexivity.
-    * induction σ; split.
-      ** destruct a. intro. unfold "=ml".
-         eapply useGenericReasoning.
-         apply pile_any.
-         mlFreshEvar as x.
-         mlFreshEvar as y.
-         mlFreshEvar as z.
-         eapply (floor_is_predicate _ _ AnyReasoning x y z).
-         3: fm_solve.
-         3: fm_solve.
-         3: fm_solve.
-         3: try_solve_pile.
-         assumption.
-         wf_auto2.
-      ** apply IHσ...
-    * intros [] ? ? ? ?.
-      (* destruct a. *)
-      eenough (well_formed _).
-      eenough (well_formed _).
-      pose proof (predicate_and Γ _ _ HΓ H3 H2).
-      apply (MP (H H3)) in H4.
-      apply (MP (H0 H2)) in H4.
-      exact H4.
-      all: wf_auto2.
-    * apply (wf_foldr) with (t := snd); only 3: intros ? [] ? ?...
-    * exact X.
-  Defined.
-
-  (* Similar proof as in Definedness_ProofSystem but object level. *)
-  Lemma def_of_pred_impl_pred_obj Γ ψ :
-    theory ⊆ Γ ->
-    well_formed ψ ->
-    Γ ⊢ is_predicate_pattern ψ ---> ⌈ ψ ⌉ ---> ψ.
-  Proof.
-    intros HΓ wfψ.
-    toMLGoal. wf_auto2. 
-    mlIntro "H0".
-    mlDestructOr "H0" as "H1" "H1".
-    - mlRewriteBy "H1" at 2.
-      mlClear "H1".
-      unfold patt_top. mlIntro. mlIntro. mlExactn 1.
-    - mlRewriteBy "H1" at 2.
-      mlRewriteBy "H1" at 1.
-      mlClear "H1".
-      fromMLGoal.
-      aapply bott_not_defined.
-  Defined.
-
-  Lemma extend_total_to_imp Γ p f :
-    theory ⊆ Γ ->
-    well_formed p ->
-    well_formed f ->
-    Γ ⊢ is_predicate_pattern p ---> (p ---> ⌊ f ⌋) ---> ⌊ p ---> f ⌋.
-  Proof.
-    intros HΓ Hwfp Hwff.
-    do 2 mlIntro.
-    epose proof (def_of_pred_impl_pred_obj Γ p HΓ Hwfp).
-    mlApplyMeta H in "0".
-    opose proof (syllogism Γ ⌈ p ⌉ p ⌊ f ⌋ _ Hwfp _).
-    1-2: wf_auto2. use AnyReasoning in H0.
-    mlApplyMeta H0 in "0". mlApply "0" in "1".
-    opose proof (impl_eq_or Γ ⌈ p ⌉ ⌊ f ⌋ _ _).
-    1-2: wf_auto2. use AnyReasoning in H1.
-    apply pf_iff_proj1 in H1. 2-3: wf_auto2.
-    mlApplyMeta H1 in "1".
-    epose proof (def_propagate_not Γ p HΓ Hwfp).
-    use AnyReasoning in H2.
-    mlAssert ("2" : (⌊ ! p ⌋ or ⌊ f ⌋)).
-    wf_auto2. mlRewrite <- H2 at 1. mlAssumption.
-    opose proof (patt_or_total Γ (! p) f AnyReasoning HΓ _ Hwff).
-    wf_auto2. mlApplyMeta H3 in "2".
-    epose proof (impl_eq_or Γ p f Hwfp Hwff).
-    use AnyReasoning in H4.
-    mlRewrite H4 at 1. mlAssumption.
-  Defined.
-
-  Tactic Notation "mlDeductHypo" constr(name) :=
-    match goal with
-    | [ |- context[ mkNH _ name (⌊ ?p ⌋) ] ] => 
-        match goal with
-        | [ |- context[ mkMLGoal _ ?t _ _ _ ] ] =>
-            mlDeduct name;
-            let i := fresh "i" in remember (ExGen := _, SVSubst := _, KT:= _, AKT := _) as i;
-            let H := fresh "H" in opose proof (hypothesis (t ∪ {[p]}) p _ ltac:(set_solver)) as H;
-            last first;
-            [use i in H |]
-        end
-    end.
-
-  Lemma extract_common_from_equality_r_2 Γ a b p :
-    theory ⊆ Γ ->
-    well_formed a ->
-    well_formed b ->
-    well_formed p ->
-    Γ ⊢ is_predicate_pattern p --->
-    (p ---> a =ml b) <---> (a and p) =ml (b and p).
-  Proof.
-    intros HΓ Hwfa Hwfb Hwfp.
-    mlIntro.
-    mlSplitAnd; mlIntro.
-    -
-      opose proof (extend_total_to_imp Γ p (a <---> b) HΓ Hwfp _). wf_auto2.
-      mlApplyMeta H in "0". mlApply "0" in "1".
-      mlClear "0". mlDeductHypo "1". 2: wf_auto2.
-      remember (Γ ∪ _) as Γ'.
-      epose proof (extract_common_from_equivalence_r Γ' p a b i Hwfp Hwfa Hwfb).
-      apply pf_iff_proj2 in H1. 2-3: wf_auto2.
-      apply (MP H0) in H1. mlRewrite H1 at 1. mlReflexivity.
-    -
-      mlIntro.
-      mlApplyMeta predicate_equiv in "0". 2: auto.
-      mlDestructAnd "0". mlApply "3" in "2".
-      mlClear "3". mlClear "4".
-      mlConj "1" "2" as "0".
-      mlClear "1". mlClear "2".
-      epose proof patt_total_and _ _ _ HΓ _ _.
-      use AnyReasoning in H.
-      apply pf_iff_proj2 in H.
-      mlApplyMeta H in "0". 2-3: wf_auto2. clear H.
-      mlDeductHypo "0".
-      2: wf_auto2.
-      remember (Γ ∪ _) as Γ'.
-      pose proof extract_common_from_equivalence_r Γ' p a b i Hwfp Hwfa Hwfb.
-      apply pf_iff_proj1 in H0.
-      apply lhs_from_and in H0.
-      apply (MP H) in H0.
-      mlRewrite H0 at 1. mlReflexivity.
-      Unshelve.
-      all: wf_auto2.
   Defined.
 
   Lemma Lemma₅ : forall (σ : list (evar * Pattern)) t₁ t₂ Γ,
@@ -294,9 +125,9 @@ Section unification.
     apply (MP H) in H0.
     apply pf_iff_proj2 in H0. 2,3: wf_auto2.
     mlApplyMeta H0.
-    epose proof (Lemma₂ Γ t₁ σ AnyReasoning _ _ _ _ _).
+    epose proof (Lemma₂ Γ t₁ σ _ _ _ _ _).
     mlRewrite <- H1 at 1.
-    epose proof (Lemma₂ Γ t₂ σ AnyReasoning _ _ _ _ _).
+    epose proof (Lemma₂ Γ t₂ σ _ _ _ _ _).
     mlRewrite <- H2 at 1.
     mlRewriteBy "H" at 1.
     mlReflexivity.
@@ -316,316 +147,12 @@ Section unification.
     mlReflexivity.
   Defined.
 
-  Definition WFPattern := sig well_formed.
-  Definition mkWFWrapper (f : Pattern -> Pattern -> Pattern) (wfp : forall a b, well_formed a -> well_formed b -> well_formed (f a b)) : WFPattern -> WFPattern -> WFPattern.
-  Proof.
-    intros * [a wfa] [b wfb].
-    exists (f a b). exact (wfp a b wfa wfb).
-  Defined.
-  Definition WFPatt_imp := mkWFWrapper patt_imp well_formed_imp.
-  Notation "a wf---> b"  := (WFPatt_imp a b) (at level 75, right associativity) : ml_scope.
-  Definition WFPatt_and := mkWFWrapper patt_and well_formed_and.
-  Notation "a 'wfand' b" := (WFPatt_and   a b) (at level 72, left associativity) : ml_scope.
-  Definition WFPatt_iff := mkWFWrapper patt_iff well_formed_iff.
-  Notation "a wf<---> b" := (WFPatt_iff a b) (at level 74, no associativity) : ml_scope.
-  Definition WFPatt_equal := mkWFWrapper patt_equal well_formed_equal.
-  Notation "p wf=ml q" := (WFPatt_equal p q) (at level 67) : ml_scope.
-  Definition WFFree_evar_subst (x : evar) := mkWFWrapper (flip free_evar_subst x) (fun a b => well_formed_free_evar_subst x b a).
-  Notation "e ^wf[[ 'evar:' x ↦ e' ]]" := (WFFree_evar_subst x e' e) (at level 2, e' at level 200, left associativity, format "e ^wf[[ 'evar:' x ↦ e' ]]" ) : ml_scope.
-  Definition WFDerives (Γ : Theory) (p : WFPattern) : Set := derives Γ (proj1_sig p).
-  Notation "Γ ⊢wf ϕ" := (WFDerives Γ ϕ) (at level 95, no associativity).
-  Definition WFPatt_app := mkWFWrapper patt_app well_formed_app.
-  Notation "a wf⋅ b" := (WFPatt_app a b) (at level 66, left associativity) : ml_scope.
-  Lemma well_formed_free_evar : forall e, well_formed (patt_free_evar e).
-  Proof.
-    exact (const eq_refl).
-  Defined.
-
-  (**
-    This typeclass represents (in an abstract way) the unification problems of
-
-      Unification in Matching Logic - Extended Version
-      Andrei Arusoaie, Dorel Lucanu
-      https://arxiv.org/abs/1811.02835v3
-
-      In the following description, we highlight the connection to this paper.
-  *)
-  Class UP (T : Type) := {
-    (** Insertion operation:
-
-          insertUP P (t, u) ~ P ∪ {t ≐ u}
-      *)
-    insertUP : T -> (WFPattern * WFPattern) -> T;
-    (** Failed unification problem
-
-          bottomUP ~ ⊥
-      *)
-
-    bottomUP : T;
-    (** Conversion to predicate. Expected to be conjunction of equalities.
-
-          toPredicateUP P ~ ϕᴾ
-      *)
-
-    toPredicateUP : T -> WFPattern;
-    (** Substitution of a variable to a pattern in every pattern of
-        a unification problem
-
-          substituteAllUP x t P ~ P{x ↦ t}
-      *)
-
-    substituteAllUP : evar -> WFPattern -> T -> T;
-    (** Creation of a singleton problem
-
-          singletonUP t u ~ {t ≐ u}
-      *)
-
-    singletonUP : WFPattern -> WFPattern -> T;
-
-    (**
-      Converting a unification problem maps insertion to conjunction.
-     *)
-    toPredicateInsertUP : forall Γ t x y, Γ ⊢wf toPredicateUP (insertUP t (x, y)) wf<---> ((x wf=ml y) wfand (toPredicateUP t));
-
-    (**
-      Converting a unification problem maps substitution of unification problems
-      to substitution of patterns.
-     *)
-    toPredicateSubstituteAllUP : forall Γ t e p, Γ ⊢wf toPredicateUP (substituteAllUP e p t) wf<---> (toPredicateUP t)^wf[[evar:e↦p]];
-
-    (**
-      Inserting into a non-⊥ unification problem cannot result ⊥.
-     *)
-    insertNotBottomUP : forall t x, t ≠ bottomUP -> insertUP t x ≠ bottomUP;
-
-    (**
-      Converting a singleton problem to a predicate pattern gives us an equality.
-     *)
-    toPredicateSingletonUP : forall Γ t1 t2, Γ ⊢wf toPredicateUP (singletonUP t1 t2) wf<---> (t1 wf=ml t2)
-  }.
-
-  Lemma lift_derives : forall Γ p, derives Γ (proj1_sig p) -> WFDerives Γ p.
-  Proof.
-    intros. auto.
-  Defined.
-
-  Lemma unwrap_wfwrapper : forall f wff a b, proj1_sig (mkWFWrapper f wff a b) = f (`a) (`b).
-  Proof.
-    now intros ? ? [a wfa] [b wfb].
-  Defined.
-
-  Lemma wfWFPattern : forall (p : WFPattern), well_formed (proj1_sig p).
-  Proof.
-    intros [p wfp]. exact wfp.
-  Defined.
-
-  Tactic Notation "mlDestructBotDocVer" := match goal with [ |- context [mkNH _ ?x patt_bott] ] => mlDestructBot x end.
-
-  Tactic Notation "refine_wf" := repeat first [
-      apply well_formed_imp |
-      apply well_formed_and |
-      apply well_formed_equal |
-      apply well_formed_free_evar_subst |
-      apply well_formed_top |
-      apply well_formed_free_evar
-    ].
-
-  Tactic Notation "mlDecomposeAll" := do !
-    match goal with
-    | [ |- context[(mkMLGoal _ _ _ (patt_imp _ _) _)] ] => mlIntro
-    | [ |- context[mkNH _ ?x (patt_and _ _)] ] => mlDestructAnd x
-    end.
-
-  Lemma set_fold_disj_union_strong_equiv `{FinSet A C} Γ (f : A → WFPattern → WFPattern) (b : WFPattern) (X Y : C) :
-  (∀ x1 x2 b',
-  x1 ∈ X ∪ Y → x2 ∈ X ∪ Y → x1 ≠ x2 →
-  Γ ⊢wf (f x1 (f x2 b')) wf<---> (f x2 (f x1 b'))) →
-  X ## Y →
-  Γ ⊢wf (set_fold f b (X ∪ Y)) wf<---> (set_fold f (set_fold f b X) Y).
-  Admitted.
-  (* Proof. *)
-  (*   intros Hf Hdisj. unfold set_fold; simpl. *)
-  (*   rewrite <- foldr_app. *)
-  (*   epose proof foldr_permutation. *)
-  (*   apply (foldr_permutation R f b). *)
-  (*   - intros j1 x1 j2 x2 b' Hj Hj1 Hj2. apply Hf. *)
-  (*     + apply elem_of_list_lookup_2 in Hj1. set_solver. *)
-  (*     + apply elem_of_list_lookup_2 in Hj2. set_solver. *)
-  (*     + intros →. pose proof (NoDup_elements (X ∪ Y)). *)
-  (*       by eapply Hj, NoDup_lookup. *)
-  (*   - by rewrite elements_disj_union, (comm (++)). *)
-  (* Qed. *)
-
-  Lemma in_set_implies_in_predicate `{FinSet A C} `{!LeibnizEquiv C} : forall Γ f b x (X : C), x ∈ X -> Γ ⊢wf set_fold (WFPatt_and ∘ f) b X wf---> f x.
-  Proof.
-    intros.
-    opose proof* (set_ind' (fun X' => Γ ⊢wf set_fold (WFPatt_and ∘ f) b ({[x]} ∪ X') wf---> f x) _ _ X).
-    rewrite -> union_empty_r_L, set_fold_singleton. simpl.
-    unfold WFDerives. toMLGoal. apply wfWFPattern. rewrite ! unwrap_wfwrapper. mlDecomposeAll; mlAssumption.
-    intros.
-    rewrite union_assoc_L.
-    destruct (EqDecision0 x x0) as [-> | ].
-    rewrite union_idemp_L. exact H9.
-    rewrite -> (union_comm_L {[x]}), <- union_assoc_L, union_comm_L.
-    opose proof* (set_fold_disj_union_strong_equiv Γ (WFPatt_and ∘ f) b ({[x]} ∪ X0) {[x0]} _ _).
-    intros. simpl.
-    unfold WFDerives. toMLGoal. apply wfWFPattern. rewrite ! unwrap_wfwrapper.
-    mlSplitAnd; mlDecomposeAll; repeat mlSplitAnd; mlAssumption.
-    set_solver.
-    rewrite set_fold_singleton in H10. simpl in H10.
-    unfold WFDerives in H10, H9 |- *.
-    toMLGoal. apply wfWFPattern.
-    rewrite ! unwrap_wfwrapper in H10, H9 |- *.
-    mlIntro. apply pf_iff_proj1 in H10. mlApplyMeta H10 in "0".
-    mlDestructAnd "0". mlApplyMeta H9 in "2". mlAssumption.
-    1-2: refine_wf; apply wfWFPattern.
-    simpl in H8.
-    apply elem_of_subseteq_singleton in H7.
-    apply subseteq_union_1_L in H7.
-    rewrite H7 in H8. exact H8.
-  Defined.
-
-  Lemma WFPattern_eq_dec : EqDecision (WFPattern * WFPattern).
-  Proof.
-    apply @prod_eq_dec.
-    all: apply sig_eq_dec.
-    1, 3: intros; apply eq_pi; apply decide_rel; apply bool_eq_dec.
-    1, 2: apply Pattern_eqdec.
-  Defined.
-
-  #[refine] Instance optionSetUP `{H : ElemOf (WFPattern * WFPattern) T, H0 : Empty T, H1 : Singleton (WFPattern * WFPattern) T, H2 : Union T, H3 : Intersection T, H4 : Difference T, H5 : Elements (WFPattern * WFPattern) T, @FinSet (WFPattern * WFPattern) T H H0 H1 H2 H3 H4 H5 WFPattern_eq_dec, !LeibnizEquiv T} : UP (option T) := {
-    insertUP t x := option_map ({[x]} ∪.) t;
-    bottomUP := None;
-    toPredicateUP := from_option (set_fold (WFPatt_and ∘ (fun '(x, y) => x wf=ml y)) (Top ↾ well_formed_top)) (patt_bott ↾ well_formed_bott);
-    substituteAllUP e p := option_map (set_map (fun '(x, y) => (x^wf[[evar:e↦p]], y^wf[[evar:e↦p]])));
-    singletonUP t1 t2 := Some {[(t1, t2)]}
-  }.
-  Proof.
-    * intros. destruct_with_eqn t; simpl.
-      ** match goal with [ |- context[set_fold (WFPatt_and ∘ ?f') ?b' _] ] => remember f' as f; remember b' as b end.
-         epose proof (elem_of_dec_slow (x, y) t0) as [].
-         pose proof (in_set_implies_in_predicate Γ f b _ _ e).
-         rewrite subseteq_union_1_L. set_solver.
-         unfold WFDerives in H7 |- *. toMLGoal. apply wfWFPattern.
-         rewrite ! unwrap_wfwrapper in H7 |- *.
-         mlSplitAnd; mlDecomposeAll.
-         mlSplitAnd. subst f. rewrite unwrap_wfwrapper in H7.
-         mlApplyMeta H7. 1-3: mlAssumption.
-         rewrite union_comm_L.
-         opose proof* (set_fold_disj_union_strong_equiv Γ (WFPatt_and ∘ f) b t0 {[(x, y)]} _ _).
-         intros. subst f. simpl. do ! case_match.
-         unfold WFDerives. toMLGoal. apply wfWFPattern. rewrite ! unwrap_wfwrapper.
-         mlSplitAnd; mlDecomposeAll; repeat mlSplitAnd; mlAssumption.
-         set_solver.
-         rewrite set_fold_singleton in H7. simpl in H7. subst f.
-         exact H7.
-      ** unfold WFDerives. case_match. simpl.
-         apply (f_equal proj1_sig) in H7. rewrite ! unwrap_wfwrapper in H7. simpl in H7.
-         rewrite <- H7. toMLGoal. refine_wf; apply wfWFPattern.
-         mlSplitAnd; mlDecomposeAll; mlDestructBotDocVer.
-    * intros. destruct_with_eqn t; simpl.
-      ** match goal with [ |- context[set_fold (WFPatt_and ∘ ?f') ?b' (set_map ?g' _)] ] => remember f' as f; remember b' as b; remember g' as g end.
-         apply (set_fold_ind' (fun r X => Γ ⊢wf set_fold (WFPatt_and ∘ f) b (set_map g X) wf<---> r^wf[[evar:e↦p]]) (WFPatt_and ∘ f) b).
-         rewrite -> set_map_empty, set_fold_empty. subst b.
-         unfold WFDerives. rewrite ! unwrap_wfwrapper. simpl.
-         toMLGoal. wf_auto2. mlSplitAnd; mlDecomposeAll.
-         mlAssumption. pose proof (top_holds Γ). use AnyReasoning in H7. mlExactMeta H7.
-         intros. simpl. rewrite -> set_map_union_L, set_map_singleton_L.
-         unshelve epose proof (elem_of_dec_slow (g x) (set_map g X)) as [].
-         1: exact T. 4: exact H6. 1-3: auto.
-         rewrite subseteq_union_1_L. apply elem_of_subseteq_singleton. exact e0.
-         epose proof (in_set_implies_in_predicate Γ f b _ _ e0).
-         unfold WFDerives in H8, H9 |- *. toMLGoal. apply wfWFPattern.
-         rewrite ! unwrap_wfwrapper in H8, H9 |- *.
-         cbn [flip] in H8 |- *. mlSimpl.
-         mlSplitAnd; mlDecomposeAll. mlSplitAnd.
-         mlApplyMeta H9 in "0". subst f g. case_match.
-         rewrite ! unwrap_wfwrapper. cbn [flip]. mlSimpl.
-         mlAssumption.
-         apply pf_iff_proj1 in H8. mlApplyMeta H8. mlAssumption.
-         1-2: refine_wf; apply wfWFPattern.
-         apply pf_iff_proj2 in H8. mlApplyMeta H8. mlAssumption.
-         1-2: refine_wf; apply wfWFPattern.
-         rewrite union_comm_L.
-         unshelve opose proof* (set_fold_disj_union_strong_equiv Γ (WFPatt_and ∘ f) b (set_map g X) {[g x]}).
-         5: exact H6. all: auto.
-         intros.
-         subst f g. simpl. repeat case_match.
-         unfold WFDerives. toMLGoal. apply wfWFPattern.
-         rewrite ! unwrap_wfwrapper. mlSplitAnd; mlDecomposeAll;
-         repeat mlSplitAnd; mlAssumption.
-         set_solver.
-         unfold WFDerives in H9, H8 |- *.
-         rewrite ! unwrap_wfwrapper in H9, H8 |- *.
-         cbn [flip] in H8 |- *.
-         eapply pf_iff_equiv_trans. 4: exact H9.
-         1-3: refine_wf; apply wfWFPattern.
-         rewrite set_fold_singleton. cbn [compose].
-         mlSimpl. rewrite unwrap_wfwrapper.
-         toMLGoal. refine_wf; apply wfWFPattern.
-         mlSplitAnd; mlDecomposeAll; mlSplitAnd.
-         subst f g. case_match. rewrite ! unwrap_wfwrapper.
-         cbn [flip]. mlSimpl. mlAssumption.
-         apply pf_iff_proj1 in H8. mlApplyMeta H8. mlAssumption.
-         1-2: refine_wf; apply wfWFPattern.
-         subst f g. case_match. rewrite ! unwrap_wfwrapper.
-         cbn [flip]. mlSimpl. mlAssumption.
-         apply pf_iff_proj2 in H8. mlApplyMeta H8. mlAssumption.
-         1-2: refine_wf; apply wfWFPattern.
-      ** case_match. apply (f_equal proj1_sig) in H7. rewrite unwrap_wfwrapper in H7. simpl in H7. unfold WFDerives. simpl. rewrite H7. now aapply pf_iff_equiv_refl.
-    * intros. destruct_with_eqn t. simpl. discriminate. now destruct H7.
-    * intros. simpl. rewrite set_fold_singleton. simpl.
-      unfold WFDerives. rewrite ! unwrap_wfwrapper. simpl.
-      toMLGoal. refine_wf; apply wfWFPattern.
-      mlSplitAnd; mlDecomposeAll; only 2: mlSplitAnd; try mlAssumption.
-      pose proof (top_holds Γ). use AnyReasoning in H7.
-      mlExactMeta H7.
-  Defined.
-
-  Reserved Notation "P ===> P'" (at level 80).
-  Inductive unification_step {T : Set} {UPT : UP T} : T -> T -> Set :=
-    | deleteUS : forall P t,
-        P ≠ bottomUP ->
-        insertUP P (t, t) ===> P
-    | decompositionUS : forall P f t g u,
-        P ≠ bottomUP ->
-        insertUP P (f wf⋅ t, g wf⋅ u) ===> insertUP (insertUP P (f, g)) (t, u)
-    | symbol_clash_lUS : forall P f t,
-        P ≠ bottomUP ->
-        patt_sym f ≠ `t ->
-        (forall x, `t ≠ patt_free_evar x) ->
-        insertUP P (patt_sym f ↾ well_formed_sym f, t) ===> bottomUP
-    | symbol_clash_rUS : forall P f t,
-        P ≠ bottomUP ->
-        patt_sym f ≠ `t ->
-        (forall x, `t ≠ patt_free_evar x) ->
-        insertUP P (t, patt_sym f ↾ well_formed_sym f) ===> bottomUP
-    | orientUS : forall P x y,
-        P ≠ bottomUP ->
-        insertUP P (x, patt_free_evar y ↾ well_formed_free_evar y) ===> insertUP P (patt_free_evar y ↾ well_formed_free_evar y, x)
-    | occours_checkUS : forall P x t,
-        P ≠ bottomUP ->
-        x ∈ free_evars (`t) ->
-        insertUP P (patt_free_evar x ↾ well_formed_free_evar x, t) ===> bottomUP
-    | eliminationUS : forall P x t,
-        P ≠ bottomUP ->
-        x ∉ free_evars (`t) ->
-        mu_free (`t) ->
-        insertUP P (patt_free_evar x ↾ well_formed_free_evar x, t) ===> insertUP (substituteAllUP x t P) (patt_free_evar x ↾ well_formed_free_evar x, t)
-  where "P ===> P'" := (unification_step P P').
-
   (**
     TODO: this axiom should be placed into Γ later, and we have to use `hypothesis`
           to obtain it. For this, we have to create a spec. for unification/term
           algebras.
   *)
   Axiom injectivity : forall Γ f t g u, Γ ⊢ (f ⋅ t) =ml (g ⋅ u) ---> (f =ml g) and (t =ml u).
-
-  Tactic Notation "inside" tactic(inside) "outside" tactic(outside) :=
-    match goal with
-    | [ |- of_MLGoal _ ] => inside
-    | _ => outside
-    end.
 
   Lemma Lemma₃ {T : Set} {UPT : UP T} Γ P P' : theory ⊆ Γ -> P ===> P' -> P' <> bottomUP -> Γ ⊢wf toPredicateUP P wf---> toPredicateUP P'.
   Proof with inside mlClear "_" outside try apply wfWFPattern.
@@ -690,7 +217,7 @@ Section unification.
       rewrite ! unwrap_wfwrapper in H1. simpl in H1.
       pose proof (projT2 t). simpl in H2.
       mlRewrite H1 at 1. clear H2.
-      opose proof* (Lemma₂ Γ (proj1_sig (toPredicateUP P0)) [(x, projT1 t)] AnyReasoning); cbn; rewrite ? andb_true_r; auto...
+      opose proof* (Lemma₂ Γ (proj1_sig (toPredicateUP P0)) [(x, projT1 t)]); cbn; rewrite ? andb_true_r; auto...
       admit.
       simpl in H2. apply pf_iff_proj2 in H2.
       2-3: refine_wf...
@@ -704,18 +231,6 @@ Section unification.
       mlDestructAnd "H0" as "H1" "H2". mlDestructAnd "H2" as "H3" "_"...
       mlSplitAnd; mlAssumption.
   Admitted.
-
-  Definition compose_substitution (σ η : list (evar * Pattern)) : list (evar * Pattern) := map (fun '(e, p) => (e, substitute_list η p)) σ.
-
-  Definition more_general_substitution (σ η : list (evar * Pattern)) : Prop := exists (θ : list (evar * Pattern)), compose_substitution σ θ = η.
-
-  Definition is_most_general_unifier_of (σ : list (evar * Pattern)) (t₁ t₂ : Pattern) : Type := (forall Γ, Γ ⊢ is_unifier_of σ t₁ t₂) * (forall η, more_general_substitution σ η).
-
-  (* NOTE Could I make US a Prop and use stdpp's rtc for this? *)
-  Inductive USrtc {T : Set} {UPT : UP T} : T -> T -> Set :=
-    | USrtc_last : forall a, USrtc a a
-    | USrtc_step : forall a b c, a ===> b -> USrtc b c -> USrtc a c
-  .
 
   (**
     The formalized unification algorithm gives us an MGU.
@@ -755,7 +270,7 @@ Section unification.
     is_most_general_unifier_of σ (`t1) (`t2) -> Γ ⊢ `t1 =ml `t2 ---> predicate_list σ.
   Proof with try apply wfWFPattern.
     intros * HΓ WFσ HMGU.
-    opose proof* (@optionSetUP (gset (WFPattern * WFPattern))).
+    opose proof* (@optionSetUP _ _ (gset (WFPattern * WFPattern))).
     1-2: typeclasses eauto.
     pose proof (convenient σ t1 t2 HMGU) as [P [[R NB] EQ] ].
     toMLGoal. simpl. refine_wf...
@@ -837,10 +352,6 @@ Section unification.
     all: mlRewrite H1 at 1; mlReflexivity.
   Defined.
 
-  Tactic Notation "mlConjFast" constr(a) constr(b) "as" constr(c) "wfby" tactic(d) := match goal with | [ |- context[mkNH _ a ?x] ] => match goal with | [ |- context[mkNH _ b ?y] ] => mlAssert (c : (x and y)); [d | mlSplitAnd; [mlExact a | mlExact b] |] end end.
-
-  Tactic Notation "mlConjFast" constr(a) constr(b) "as" constr(c) := mlConjFast a b as c wfby idtac.
-
   Goal forall Γ (f' g' one' : symbols) (x' y' z' : evar) (*one : WFPattern*),
     x' ≠ z' -> y' ≠ z' ->
     theory ⊆ Γ ->
@@ -888,7 +399,7 @@ Section unification.
     {
       mlApplyMeta H in "0".
       pose proof (@gset_fin_set _ WFPattern_eq_dec ltac:(typeclasses eauto)).
-      pose (@optionSetUP _ _ _ _ _ _ _ _ H0 ltac:(typeclasses eauto)).
+      pose (@optionSetUP _ _ _ _ _ _ _ _ _ _ H0 ltac:(typeclasses eauto)).
       opose proof* (Lemma₄_helper Γ (Some (singleton (t1, t2)))). auto.
       eright. pose proof (decompositionUS (Some empty)). simpl in H1. rewrite <- union_empty_r_L. apply H1... rewrite union_empty_r_L.
       eright. epose proof (decompositionUS (Some _)). simpl in H1. apply H1...
@@ -935,7 +446,7 @@ Section unification.
       mlExact "1".
     }
     {
-      opose proof* (Lemma₂ Γ (`t1) σ AnyReasoning)...
+      opose proof* (Lemma₂ Γ (`t1) σ)...
       opose proof* (wf_substitute_list σ (`t1))...
       apply pf_iff_proj2 in H... mlSplitAnd. mlDestructAnd "0"; mlAssumption.
       mlApplyMeta H in "0". unfold t1. simpl.
