matching-logic/src/Experimental/Unification/Helpers.v
@@ -1,0 +1,211 @@
+From MatchingLogic.Theories Require Export FOEquality_ProofSystem.
+Import MatchingLogic.Logic.Notations.
+Import MatchingLogic.Theories.Definedness_Syntax.Notations.
+
+From MatchingLogic Require Export Unification.TacticsNotations.
+
+Set Default Proof Mode "Classic".
+
+Close Scope equations_scope. (* Because of [!] *)
+
+Section Helpers.
+  Context {Σ : Signature} {syntax : Syntax}.
+
+  Definition get_fresh_evar (φ : Pattern) : sig (.∉ free_evars φ).
+  Proof.
+    exists (fresh_evar φ); auto.
+  Defined.
+
+  Definition substitute_list (σ : list (evar * Pattern)) (t : Pattern) : Pattern := fold_left (fun φ '(x, φ') => φ^[[evar: x ↦ φ']]) σ t.
+
+  Lemma wf_substitute_list : forall σ t, wf (map snd σ) -> well_formed t -> well_formed (substitute_list σ t).
+  Proof.
+    intros.
+    apply wf_fold_left with (t := snd); try assumption.
+    intros ? [] **; wf_auto2.
+  Qed.
+
+  Definition predicate_list (σ : list (evar * Pattern)) : Pattern := fold_right (fun '(x, φ') φ => patt_free_evar x =ml φ' and φ) patt_top σ.
+
+  Lemma wf_predicate_list : forall σ, wf (map snd σ) -> well_formed (predicate_list σ).
+  Proof.
+    intros.
+    apply wf_foldr with (t := snd);
+    only 3: intros ? [] **; wf_auto2.
+  Qed.
+  
+  Lemma predicate_list_predicate Γ σ : theory ⊆ Γ -> wf (map snd σ) -> Γ ⊢ is_predicate_pattern (predicate_list σ).
+  Proof with wf_auto2.
+    intros HΓ wfσ.
+    epose proof (foldr_ind_set (λ φ, well_formed φ -> Γ ⊢ is_predicate_pattern φ) (λ '(x, φ), well_formed (patt_free_evar x =ml φ) -> Γ ⊢ is_predicate_pattern (patt_free_evar x =ml φ)) (λ '(x, φ') (φ : Pattern), patt_free_evar x =ml φ' and φ) patt_top σ).
+    ospecialize* X. 1-4: clear X.
+    * intro. toMLGoal... mlLeft. mlReflexivity.
+    * induction σ; split.
+      ** destruct a. intro. unfold "=ml".
+         eapply useGenericReasoning.
+         apply pile_any.
+         mlFreshEvar as x.
+         mlFreshEvar as y.
+         mlFreshEvar as z.
+         eapply (floor_is_predicate _ _ AnyReasoning x y z).
+         3: fm_solve.
+         3: fm_solve.
+         3: fm_solve.
+         3: try_solve_pile.
+         assumption.
+         wf_auto2.
+      ** apply IHσ...
+    * intros [] ? ? ? ?.
+      (* destruct a. *)
+      eenough (well_formed _).
+      eenough (well_formed _).
+      pose proof (predicate_and Γ _ _ HΓ H3 H2).
+      apply (MP (H H3)) in H4.
+      apply (MP (H0 H2)) in H4.
+      exact H4.
+      all: wf_auto2.
+    * apply (wf_foldr) with (t := snd); only 3: intros ? [] ? ?...
+    * exact X.
+  Defined.
+
+  (* Similar proof as in Definedness_ProofSystem but object level. *)
+  Lemma def_of_pred_impl_pred_obj Γ ψ :
+    theory ⊆ Γ ->
+    well_formed ψ ->
+    Γ ⊢ is_predicate_pattern ψ ---> ⌈ ψ ⌉ ---> ψ.
+  Proof.
+    intros HΓ wfψ.
+    toMLGoal. wf_auto2. 
+    mlIntro "H0".
+    mlDestructOr "H0" as "H1" "H1".
+    - mlRewriteBy "H1" at 2.
+      mlClear "H1".
+      unfold patt_top. mlIntro. mlIntro. mlExactn 1.
+    - mlRewriteBy "H1" at 2.
+      mlRewriteBy "H1" at 1.
+  mlClear "H1".
+  fromMLGoal.
+  aapply bott_not_defined.
+  Defined.
+
+  Lemma extend_total_to_imp Γ p f :
+    theory ⊆ Γ ->
+    well_formed p ->
+    well_formed f ->
+    Γ ⊢ is_predicate_pattern p ---> (p ---> ⌊ f ⌋) ---> ⌊ p ---> f ⌋.
+  Proof.
+    intros HΓ Hwfp Hwff.
+    do 2 mlIntro.
+    epose proof (def_of_pred_impl_pred_obj Γ p HΓ Hwfp).
+    mlApplyMeta H in "0".
+    opose proof (syllogism Γ ⌈ p ⌉ p ⌊ f ⌋ _ Hwfp _).
+    1-2: wf_auto2. use AnyReasoning in H0.
+    mlApplyMeta H0 in "0". mlApply "0" in "1".
+    opose proof (impl_eq_or Γ ⌈ p ⌉ ⌊ f ⌋ _ _).
+    1-2: wf_auto2. use AnyReasoning in H1.
+    apply pf_iff_proj1 in H1. 2-3: wf_auto2.
+    mlApplyMeta H1 in "1".
+    epose proof (def_propagate_not Γ p HΓ Hwfp).
+    use AnyReasoning in H2.
+    mlAssert ("2" : (⌊ ! p ⌋ or ⌊ f ⌋)).
+    wf_auto2. mlRewrite <- H2 at 1. mlAssumption.
+    opose proof (patt_or_total Γ (! p) f AnyReasoning HΓ _ Hwff).
+    wf_auto2. mlApplyMeta H3 in "2".
+    epose proof (impl_eq_or Γ p f Hwfp Hwff).
+    use AnyReasoning in H4.
+    mlRewrite H4 at 1. mlAssumption.
+  Defined.
+
+  Lemma extract_common_from_equality_r_2 Γ a b p :
+    theory ⊆ Γ ->
+    well_formed a ->
+    well_formed b ->
+    well_formed p ->
+    Γ ⊢ is_predicate_pattern p --->
+    (p ---> a =ml b) <---> (a and p) =ml (b and p).
+  Proof.
+    intros HΓ Hwfa Hwfb Hwfp.
+    mlIntro.
+    mlSplitAnd; mlIntro.
+    -
+      opose proof (extend_total_to_imp Γ p (a <---> b) HΓ Hwfp _). wf_auto2.
+      mlApplyMeta H in "0". mlApply "0" in "1".
+      mlClear "0". mlDeductHypo "1". 2: wf_auto2.
+      remember (Γ ∪ _) as Γ'.
+      epose proof (extract_common_from_equivalence_r Γ' p a b i Hwfp Hwfa Hwfb).
+      apply pf_iff_proj2 in H1. 2-3: wf_auto2.
+      apply (MP H0) in H1. mlRewrite H1 at 1. mlReflexivity.
+    -
+      mlIntro.
+      mlApplyMeta predicate_equiv in "0". 2: auto.
+      mlDestructAnd "0". mlApply "3" in "2".
+      mlClear "3". mlClear "4".
+      mlConj "1" "2" as "0".
+      mlClear "1". mlClear "2".
+      epose proof patt_total_and _ _ _ HΓ _ _.
+      use AnyReasoning in H.
+      apply pf_iff_proj2 in H.
+      mlApplyMeta H in "0". 2-3: wf_auto2. clear H.
+      mlDeductHypo "0".
+      2: wf_auto2.
+      remember (Γ ∪ _) as Γ'.
+      pose proof extract_common_from_equivalence_r Γ' p a b i Hwfp Hwfa Hwfb.
+      apply pf_iff_proj1 in H0.
+      apply lhs_from_and in H0.
+      apply (MP H) in H0.
+      mlRewrite H0 at 1. mlReflexivity.
+      Unshelve.
+      all: wf_auto2.
+  Defined.
+
+Lemma set_fold_disj_union_strong_equiv `{FinSet A C} Γ (f : A → WFPattern → WFPattern) (b : WFPattern) (X Y : C) :
+(∀ x1 x2 b',
+x1 ∈ X ∪ Y → x2 ∈ X ∪ Y → x1 ≠ x2 →
+Γ ⊢wf (f x1 (f x2 b')) wf<---> (f x2 (f x1 b'))) →
+X ## Y →
+Γ ⊢wf (set_fold f b (X ∪ Y)) wf<---> (set_fold f (set_fold f b X) Y).
+Admitted.
+(* Proof. *)
+(*   intros Hf Hdisj. unfold set_fold; simpl. *)
+(*   rewrite <- foldr_app. *)
+(*   epose proof foldr_permutation. *)
+(*   apply (foldr_permutation R f b). *)
+(*   - intros j1 x1 j2 x2 b' Hj Hj1 Hj2. apply Hf. *)
+(*     + apply elem_of_list_lookup_2 in Hj1. set_solver. *)
+(*     + apply elem_of_list_lookup_2 in Hj2. set_solver. *)
+(*     + intros →. pose proof (NoDup_elements (X ∪ Y)). *)
+(*       by eapply Hj, NoDup_lookup. *)
+(*   - by rewrite elements_disj_union, (comm (++)). *)
+(* Qed. *)
+
+Lemma in_set_implies_in_predicate `{FinSet A C} `{!LeibnizEquiv C} : forall Γ f b x (X : C), x ∈ X -> Γ ⊢wf set_fold (WFPatt_and ∘ f) b X wf---> f x.
+Proof.
+  intros.
+  opose proof* (set_ind' (fun X' => Γ ⊢wf set_fold (WFPatt_and ∘ f) b ({[x]} ∪ X') wf---> f x) _ _ X).
+  rewrite -> union_empty_r_L, set_fold_singleton. simpl.
+  unfold WFDerives. toMLGoal. apply wfWFPattern. rewrite ! unwrap_wfwrapper. mlDecomposeAll; mlAssumption.
+  intros.
+  rewrite union_assoc_L.
+  destruct (EqDecision0 x x0) as [-> | ].
+  rewrite union_idemp_L. exact H9.
+  rewrite -> (union_comm_L {[x]}), <- union_assoc_L, union_comm_L.
+  opose proof* (set_fold_disj_union_strong_equiv Γ (WFPatt_and ∘ f) b ({[x]} ∪ X0) {[x0]} _ _).
+  intros. simpl.
+  unfold WFDerives. toMLGoal. apply wfWFPattern. rewrite ! unwrap_wfwrapper.
+  mlSplitAnd; mlDecomposeAll; repeat mlSplitAnd; mlAssumption.
+  set_solver.
+  rewrite set_fold_singleton in H10. simpl in H10.
+  unfold WFDerives in H10, H9 |- *.
+  toMLGoal. apply wfWFPattern.
+  rewrite ! unwrap_wfwrapper in H10, H9 |- *.
+  mlIntro. apply pf_iff_proj1 in H10. mlApplyMeta H10 in "0".
+  mlDestructAnd "0". mlApplyMeta H9 in "2". mlAssumption.
+  1-2: refine_wf; apply wfWFPattern.
+  simpl in H8.
+  apply elem_of_subseteq_singleton in H7.
+  apply subseteq_union_1_L in H7.
+  rewrite H7 in H8. exact H8.
+Defined.
+
+End Helpers.
+
