matching-logic/src/Experimental/Unification/TacticsNotations.v
@@ -1,0 +1,102 @@
+From MatchingLogic.Theories Require Export FOEquality_ProofSystem.
+Import MatchingLogic.Logic.Notations.
+Import MatchingLogic.Theories.Definedness_Syntax.Notations.
+
+Set Default Proof Mode "Classic".
+
+Close Scope equations_scope. (* Because of [!] *)
+
+Section TacticsNotations.
+  Context {Σ : Signature} {syntax : Syntax}.
+
+  Definition WFPattern := sig well_formed.
+  Definition mkWFWrapper (f : Pattern -> Pattern -> Pattern) (wfp : forall a b, well_formed a -> well_formed b -> well_formed (f a b)) : WFPattern -> WFPattern -> WFPattern.
+  Proof.
+    intros * [a wfa] [b wfb].
+    exists (f a b). exact (wfp a b wfa wfb).
+  Defined.
+  Definition WFPatt_imp := mkWFWrapper patt_imp well_formed_imp.
+  Definition WFPatt_and := mkWFWrapper patt_and well_formed_and.
+  Definition WFPatt_iff := mkWFWrapper patt_iff well_formed_iff.
+  Definition WFPatt_equal := mkWFWrapper patt_equal well_formed_equal.
+  Definition WFFree_evar_subst (x : evar) := mkWFWrapper (flip free_evar_subst x) (fun a b => well_formed_free_evar_subst x b a).
+  Definition WFDerives (Γ : Theory) (p : WFPattern) : Set := derives Γ (proj1_sig p).
+  Definition WFPatt_app := mkWFWrapper patt_app well_formed_app.
+  Lemma well_formed_free_evar : forall e, well_formed (patt_free_evar e).
+  Proof.
+    exact (const eq_refl).
+  Defined.
+
+  Lemma lift_derives : forall Γ p, derives Γ (proj1_sig p) -> WFDerives Γ p.
+  Proof.
+    intros. auto.
+  Defined.
+
+  Lemma unwrap_wfwrapper : forall f wff a b, proj1_sig (mkWFWrapper f wff a b) = f (`a) (`b).
+  Proof.
+    now intros ? ? [a wfa] [b wfb].
+  Defined.
+
+  Lemma wfWFPattern : forall (p : WFPattern), well_formed (proj1_sig p).
+  Proof.
+    intros [p wfp]. exact wfp.
+  Defined.
+
+  Lemma WFPattern_eq_dec : EqDecision (WFPattern * WFPattern).
+  Proof.
+    apply @prod_eq_dec.
+    all: apply sig_eq_dec.
+    1, 3: intros; apply eq_pi; apply decide_rel; apply bool_eq_dec.
+    1, 2: apply Pattern_eqdec.
+  Defined.
+
+End TacticsNotations.
+
+Notation "a wf---> b"  := (WFPatt_imp a b) (at level 75, right associativity) : ml_scope.
+Notation "a 'wfand' b" := (WFPatt_and   a b) (at level 72, left associativity) : ml_scope.
+Notation "a wf<---> b" := (WFPatt_iff a b) (at level 74, no associativity) : ml_scope.
+Notation "p wf=ml q" := (WFPatt_equal p q) (at level 67) : ml_scope.
+Notation "e ^wf[[ 'evar:' x ↦ e' ]]" := (WFFree_evar_subst x e' e) (at level 2, e' at level 200, left associativity, format "e ^wf[[ 'evar:' x ↦ e' ]]" ) : ml_scope.
+Notation "Γ ⊢wf ϕ" := (WFDerives Γ ϕ) (at level 95, no associativity).
+Notation "a wf⋅ b" := (WFPatt_app a b) (at level 66, left associativity) : ml_scope.
+
+Tactic Notation "mlDeductHypo" constr(name) :=
+  match goal with
+  | [ |- context[ mkNH _ name (⌊ ?p ⌋) ] ] => 
+      match goal with
+      | [ |- context[ mkMLGoal _ ?t _ _ _ ] ] =>
+          mlDeduct name;
+          let i := fresh "i" in remember (ExGen := _, SVSubst := _, KT:= _, AKT := _) as i;
+          let H := fresh "H" in opose proof (hypothesis (t ∪ {[p]}) p _ ltac:(set_solver)) as H;
+          last first;
+          [use i in H |]
+      end
+  end.
+
+Tactic Notation "mlDestructBotDocVer" := match goal with [ |- context [mkNH _ ?x patt_bott] ] => mlDestructBot x end.
+
+Tactic Notation "refine_wf" := repeat first [
+  apply well_formed_imp |
+  apply well_formed_and |
+  apply well_formed_equal |
+  apply well_formed_free_evar_subst |
+  apply well_formed_top |
+  apply well_formed_free_evar
+  ].
+
+Tactic Notation "mlDecomposeAll" := do !
+  match goal with
+  | [ |- context[(mkMLGoal _ _ _ (patt_imp _ _) _)] ] => mlIntro
+  | [ |- context[mkNH _ ?x (patt_and _ _)] ] => mlDestructAnd x
+  end.
+
+Tactic Notation "inside" tactic(inside) "outside" tactic(outside) :=
+  match goal with
+  | [ |- of_MLGoal _ ] => inside
+  | _ => outside
+  end.
+
+Tactic Notation "mlConjFast" constr(a) constr(b) "as" constr(c) "wfby" tactic(d) := match goal with | [ |- context[mkNH _ a ?x] ] => match goal with | [ |- context[mkNH _ b ?y] ] => mlAssert (c : (x and y)); [d | mlSplitAnd; [mlExact a | mlExact b] |] end end.
+
+Tactic Notation "mlConjFast" constr(a) constr(b) "as" constr(c) := mlConjFast a b as c wfby idtac.
+
